\documentclass[12pt]{article}
\thispagestyle{empty}

\begin{document}

    (!) S K K = I\\
    
    Proof:\\
    
    I $\equiv$ $\lambda$x.x
    
    S $\equiv$ $\lambda$x y z.x z (y z)
    
    K $\equiv$ $\lambda$x y.x\\

    S K K $\equiv$ ($\lambda$x y z.x z (y z)) ($\lambda$x y.x) ($\lambda$x y.x)
    
    $\rightarrow_{\beta}$ ($\lambda$y z.($\lambda$x y.x) z (y z)) ($\lambda$x y.x)
    
    $\rightarrow_{\beta}$ ($\lambda$y z.($\lambda$y.z) (y z)) ($\lambda$x y.x)
    
    $\rightarrow_{\beta}$ ($\lambda$z.($\lambda$y.z) (($\lambda$x y.x) z))
    
    $\rightarrow_{\beta}$ ($\lambda$z.($\lambda$y.z) ($\lambda$y.z)))
    
    $\rightarrow_{\beta}$ ($\lambda$z.z) $\equiv$ I
    
\end{document}